src/tls/KDF.fst
@@ -23,7 +23,7 @@ module MDM = FStar.Monotonic.DependentMap
 module HS = FStar.HyperStack
 module DT = DefineTable
 
-#set-options "--max_fuel 0 --max_ifuel 0 --z3rlimit 30"
+#set-options "--max_fuel 1 --max_ifuel 1 --z3rlimit 30"
 
 (*
 This module defines a universal, packaged KDF parametric in its
@@ -49,8 +49,6 @@ type info =
   ha:kdfa ->
   option (details ha) -> info
 
-#push-options "--max_fuel 1 --max_ifuel 1"
-
 noextract
 let rec index_info (i:id{model}) =
   let i':pre_id = i in
@@ -58,8 +56,6 @@ let rec index_info (i:id{model}) =
   | Preshared a _ -> Info a None
   | Derive i l (ExpandLog log hv) -> Info (ha_of_id i) (Some (Log log hv))
   | Derive i _ _ -> index_info i
-
-#pop-options
 
 let valid_info (i:id) (v:info) = model ==> (v == index_info i)
 
@@ -75,31 +71,10 @@ let derived_key
   (lbl: label {u `has_lbl` lbl})
   (ctx: context)
   : Pure Type0
-  (requires wellformed_derive i lbl ctx /\ registered (derive i lbl ctx))
+  (requires model /\ wellformed_derive i lbl ctx /\
+    registered (derive i lbl ctx))
   (ensures fun t -> True)
-  =
-  if model then
-    Pkg?.key (child u lbl) (Derive i lbl ctx)
-  else unit
-
-let kdf_region : tls_rgn = new_region tls_tables_region
-let kdf_loc = M.loc_region_only true kdf_region
-
-/// key-derivation table (memoizing create/coerce)
-noextract
-type domain (#ideal:iflag) (u:usage ideal) (i:regid) : eqtype =
-| Domain:
-  lbl: label {u `has_lbl` lbl} ->
-  ctx: context {wellformed_derive i lbl ctx /\ registered (derive i lbl ctx)} ->
-  domain u i
-
-noextract
-let kdf_range (#ideal:iflag) (u:usage ideal) (i:regid) (d:domain u i) =
-  (let Domain lbl ctx = d in derived_key u i lbl ctx)
-
-noextract
-abstract type table (#ideal:iflag) (u:usage ideal) (i:regid) =
-  MDM.t kdf_region (domain u i) (kdf_range u i) (fun _ -> True)
+  = Pkg?.key (child u lbl) (Derive i lbl ctx)
 
 inline_for_extraction
 let secret_len (a:info) : keylen = Hashing.Spec.tagLen a.ha
@@ -108,54 +83,188 @@ type real_secret (i:regid) = a:info0 i & lbytes32 (secret_len a)
 let safe (#ideal:iflag) (u:usage ideal) (i:regid) =
   honest i /\ b2t ideal
 
+// This is the type of KDF instances
+// The idealized KDF does not have any state; 
+// we rely on the children packages to compute
+// a virtual idealization table
 type secret (#ideal:iflag) (u:usage ideal) (i:regid) =
-  Model.ir (safe u) (table u i) (real_secret i) i
+  Model.ir (safe u) unit (real_secret i) i
 
-/// Real KDF schemes, parameterized by an algorithm computed from the
-/// index (existing code).
+(* Honestly invariants for derived instances *)
 
 val lemma_witnessed_true (p:mem_predicate) :
   Lemma (requires (forall h. p h)) (ensures witnessed p)
 let lemma_witnessed_true p =
-  lemma_witnessed_constant True;
-  weaken_witness (fun _ -> True) p
+  lemma_witnessed_constant True;  weaken_witness (fun _ -> True) p
 
-#push-options "--max_ifuel 1"
-
-val lemma_honest_parent (i:regid) (lbl:label) (ctx:context)
-  : Lemma (requires
-            wellformed_derive i lbl ctx /\
-            registered (derive i lbl ctx) /\
-            ~(honest_idh ctx) /\
-            honest (derive i lbl ctx))
-          (ensures honest i)
-let lemma_honest_parent i lbl ctx =
+private let lemma_honest_parent (i:regid) (lbl:label) (ctx:context)
+  : Lemma
+  (requires wellformed_derive i lbl ctx /\ 
+    registered (derive i lbl ctx) /\ 
+    ~(honest_idh ctx) /\ 
+    honest (derive i lbl ctx))
+  (ensures honest i)
+  =
   if model then
     let log : i_honesty_table = honesty_table in
-    lemma_witnessed_true (fun h -> MDM.contains log (derive i lbl ctx) true h ==> MDM.contains log i true h);
-    lemma_witnessed_impl (MDM.contains log (derive i lbl ctx) true) (MDM.contains log i true)
-
-#pop-options
+    lemma_witnessed_true (fun h ->
+      MDM.contains log (derive i lbl ctx) true h ==> MDM.contains log i true h);
+    lemma_witnessed_impl (MDM.contains log (derive i lbl ctx) true)
+      (MDM.contains log i true)
 
 let lemma_honest_parent_impl (i:regid) (lbl:label) (ctx:context)
-  : Lemma (requires wellformed_derive i lbl ctx /\
-            registered (derive i lbl ctx) /\
-            ~(honest_idh ctx))
-          (ensures honest (derive i lbl ctx) ==> honest i)
+  : Lemma
+    (requires wellformed_derive i lbl ctx /\ 
+      registered (derive i lbl ctx) /\ ~(honest_idh ctx))
+    (ensures honest (derive i lbl ctx) ==> honest i)
   = FStar.Classical.impl_intro_gen #(honest (derive i lbl ctx)) #(fun _ -> honest i)
     (fun (u:squash (honest (derive i lbl ctx))) -> lemma_honest_parent i lbl ctx)
+
+(* Concrete info (hash agility) *)
 
 inline_for_extraction
 let get_info (#ideal:iflag) (#u:usage ideal) (#i:regid) (k:secret u i) =
   if Model.is_safe k then index_info i else dfst (Model.real k)
 
+(*** Virtual KDF table ***)
+
+(*
+The ideal behavior of a KDF is to map labels and contexts to derived instances:
+
+  ideal_kdf u i == l:label -> c:context -> k:(child u l).key (derive i l c)
+
+However, to avoid state duplication, we do not actually materialize this table.
+Instead, we compute the table from the define_table of children packages.
+This is a nice simplification because the only state of a KDF table is its own
+define table. (However, the footprint of a KDF package now includes the
+define tables of all of its children).
+
+The define table for package pkg is of the form (i:regid -> pkg.key i),
+and it is global for the package. In contrast, the KDF table is specific
+to the instance of the KDF. Hence, we need to filter the entries of children's
+define table to only the instances whose index is derived from the KDF
+instance's index. We also need to re-index the filtered table to get
+the computed idealization table.
+
+Then, we specify the security of the KDF based on operations on the virtual
+KDF table. The implementation, however, only operates on the children's
+define tables.
+*)
+
+// KDF tables are indexed by label and context
+type kdf_key (#ideal:iflag) (u:usage ideal) (i:regid{model}) (l:label{u `has_lbl` l}) =
+  c:context{wellformed_derive i l c /\ registered (derive i l c)}
+
+// They store derived instances, whose type is directed by the usage
+type kdf_value (#ideal:iflag) (u:usage ideal) (i:regid{model})
+  (l:label{u `has_lbl` l}) (k:kdf_key u i l) =
+  option (derived_key u i l k)
+
+// We shard the table by label
+type kdf_table_shard (#ideal:iflag) (u:usage ideal)
+  (i:regid{model}) (l:label{u `has_lbl` l}) =
+  DM.t (kdf_key u i l) (kdf_value u i l)
+
+// The type of computed KDF tables, indexed by label, then context
+type kdf_table (#ideal:iflag) (u:usage ideal) (i:regid{model}) =
+  DM.t (l:label{u `has_lbl` l}) (kdf_table_shard u i)
+
+type derived_from (#ideal:iflag) (u:usage ideal)
+  (i:regid{model}) (l:label{u `has_lbl` l}) (j:regid) =
+  (let j' : pre_id = j in
+  match j' with
+  | Derive i' lbl ctx -> i' == i /\ lbl == l
+  | _ -> False)
+
+// To compute the virtual KDF table, we need to re-index the
+// projection of the children's KDF tables
+let reindex (#ideal:iflag) (u:usage ideal) (i:regid{model})
+  (l:label{u `has_lbl` l}) (k:kdf_key u i l)
+  : (j:regid{derived_from u i l j}) =
+  derive i l k
+
+// This is not used concretely, but we prove that
+// the re-indexing is bijective by constructing its inverse
+let reindex_inv (#ideal:iflag) (u:usage ideal) (i:regid{model})
+  (l:label{u `has_lbl` l}) (j:regid{derived_from u i l j})
+  : kdf_key u i l =
+  let j' : pre_id = j in
+  let Derive i lbl ctx = j' in
+  ctx
+
+// We prove that the re-indexed virtual KDF table
+// is isomorphic to the filtered define table
+let lemma_reindex_correct (#ideal:iflag) (u:usage ideal)
+  (i:regid{model}) (l:label{u `has_lbl` l}) (k:kdf_key u i l)
+  : Lemma (reindex_inv u i l (reindex u i l k) == k)
+  = ()
+
+// When re-indexing the define table, we get a complicated type for the
+// renamed instances. We show this type is equivalent to kdf_value
+private noextract
+let coerce_reindex (#ideal:iflag) (u:usage ideal) (i:regid{model}) (l:label{u `has_lbl` l})
+  (k:kdf_key u i l) (v:DM.rename_value (MDM.opt (Pkg?.key (child u l))) (reindex u i l) k)
+  : kdf_value u i l k
+  = v
+
+private let lemma_has_lbl_cons (#p:Type0) (u:children' p)
+  (h:label * tree' p) (lbl:label)
+  : Lemma (requires u `has_lbl'` lbl /\ fst h <> lbl)
+  (ensures (h::u) `has_lbl'` lbl /\ child' (h::u) lbl == child' u lbl)
+  = ()
+
+// We desine a custom function for nth because we need to prove that
+// has_lbl and child are preseved by list inclusion
+private let rec nth_child (#p:Type0) (u:children' p{List.Tot.length u > 0})
+  (n:nat{model /\ n < List.Tot.length u})
+  : GTot (l:label{u `has_lbl'` l} & p:pkg ii{p == child' u l})
+  (decreases n)
+  =
+  if n = 0 then
+    let (lbl, p) = List.Tot.hd u in
+    let pkg = match p with Node p _ -> p | Leaf p -> p in
+    let _ = assert(child' u lbl == pkg) in
+    (| lbl, pkg |)
+  else 
+    let u' = List.Tot.tl u in
+    let (|lbl, p|) = nth_child u' (n-1) in
+    // FIXME(adl): label disjointness, see disjoint_labels in Pkg.Tree
+    let _ = assume(fst (List.Tot.hd u) <> lbl) in
+    let _ = lemma_has_lbl_cons u' (List.Tot.hd u) lbl in
+    (|lbl, p|)
+
+// Given the index i of a KDF instance, we compute
+// the associated virtual idealization table
+let compute_kdf_table (#ideal:iflag) (u:usage ideal) (i:regid{model}) (h:mem)
+  : GTot (kdf_table u i)
+  =
+  let l : children' (b2t ideal) = u in
+  let m = List.Tot.length l in
+  let rec aux (n:nat{n <= m}) : GTot (kdf_table u i) =
+    if n = 0 then
+      DM.create (fun l -> DM.create (fun k -> None <: kdf_value u i l k))
+    else
+      let (| lbl, pkg |) = nth_child l (m - n) in
+      let dt : DT.dt #regid (Pkg?.key (child u lbl)) = pkg.define_table in
+      // The define table is specified by a DependentMap
+      let m = MDM.repr (HS.sel h (DT.ideal dt)) in
+      // Filter for entries derived from i with label lbl
+      let m' = DM.restrict (derived_from u i lbl) m in
+      // Re-index table by context
+      let m'' = DM.rename m' (reindex u i lbl) in
+      // Coerce the type of instances to the type of KDF tables
+      let m''' = DM.map (coerce_reindex u i lbl) m'' in
+      DM.upd (aux (n-1)) lbl m'''
+    in
+  aux m
+
+(*
 type empty (#ideal:iflag) (#u:usage ideal) (#i:regid) (k:secret u i) (h:mem) =
   (if Model.is_safe k then HS.sel h (Model.ideal k) == MDM.empty else True)
 
 type live (#ideal:iflag) (#u:usage ideal) (#i:regid) (k:secret u i) (h:mem) =
   Model.is_safe k ==> h `HS.contains` (Model.ideal k)
-
-// FIXME(adl) missing the case honest_idh ctx
+*)
 
 // The KDF invariant specifies that when the KDF is ideal,
 // its table contains entries that are defined if, and only if,
@@ -173,8 +282,9 @@ type kdf_invariant_wit (#ideal:iflag) (#u:usage ideal) (#i:regid)
   let dt = DT.ideal pkg'.define_table in
   DT.live #_ #(Pkg?.key pkg') dt h /\
   (if Model.is_safe k then (
-    h `HS.contains` (Model.ideal k) /\ // KDF table is live
-    MDM.sel (sel h (Model.ideal k)) (Domain lbl ctx) == MDM.sel (sel h dt) i'
+    True
+//    h `HS.contains` (Model.ideal k) // KDF table is live
+//    MDM.sel (sel h (Model.ideal k)) (Domain lbl ctx) == MDM.sel (sel h dt) i'
   ) else
    begin
     let (| a, raw |) = Model.real k in
@@ -191,7 +301,7 @@ type kdf_invariant_wit (#ideal:iflag) (#u:usage ideal) (#i:regid)
 let lemma_kdf_invariant_init_wit (#ideal:iflag) (#u:usage ideal) (#i:regid)
   (k:secret u i) (h:mem) (lbl:label {u `has_lbl` lbl})
   (ctx:context{~(honest_idh ctx) /\ wellformed_derive i lbl ctx /\ registered (derive i lbl ctx)})
-  : Lemma (requires empty k h /\ live k h /\
+  : Lemma (requires // empty k h /\ live k h /\
     DT.live (child u lbl).define_table h /\
     DT.empty (child u lbl).define_table h)
   (ensures kdf_invariant_wit k h lbl ctx)
@@ -209,28 +319,19 @@ type kdf_invariant (#ideal:iflag) (#u:usage ideal) (#i:regid) (k:secret u i) (h:
     kdf_invariant_wit k h lbl ctx)
   else True)
 
-#push-options "--max_fuel 1 --max_ifuel 1"
-
 // The union of all the define table of the children of the KDF
-let rec children_fp (#ideal:iflag) (u:usage ideal) : GTot M.loc =
-  if model then
-    let l : children' (b2t ideal) = u in
-    match l with
-    | [] -> M.loc_none
-    | (lbl, _)::t ->
-      M.loc_union (DT.loc (child u lbl).define_table) (children_fp #ideal t)
-  else M.loc_none
-
-let loc (#ideal:iflag) (#u:usage ideal) (#i:regid) (k:secret u i) =
-  if Model.is_safe k then M.loc_mreference (Model.ideal k) else M.loc_none
+let rec children_fp (#p:Type) (u:children' p) : GTot M.loc =
+  match u with
+  | [] -> M.loc_none
+  | (lbl, _)::t ->
+    M.loc_union (DT.loc (child' u lbl).define_table) (children_fp #p t)
 
 // The footprint of the KDF invariant is:
-//  - 1. its idealized KDF table
+//  - DEPRECATED 1. its idealized KDF table
 //  - 2. the define table of all children
 let kdf_footprint (#ideal:iflag) (#u:usage ideal) (#i:regid) (k:secret u i)
-  : GTot M.loc
-  =
-  M.loc_union (loc k) (children_fp u)
+  : GTot M.loc =
+  if model then children_fp (u <: children' (b2t ideal)) else M.loc_none
 
 // Intuitively, if a location is disjoint from the KDF footprint,
 // it is disjoint from the define table of all children. The proof
@@ -244,21 +345,19 @@ let lemma_kdf_footprint_disjoint_wit (#ideal:iflag) (#u:usage ideal)
   (ensures M.loc_disjoint l (DT.loc (child u lbl).define_table))
   =
   if model then
-    let rec aux (#ideal:iflag) (u:usage ideal) (lbl:label{model /\ u `has_lbl` lbl})
+    let rec aux (#p:Type0) (u:children' p) (lbl:label{u `has_lbl'` lbl})
       : Lemma
         (requires M.loc_disjoint l (children_fp u))
-        (ensures M.loc_disjoint l (DT.loc (child u lbl).define_table))
+        (ensures M.loc_disjoint l (DT.loc (child' u lbl).define_table))
       =
-      if model then
-        let c : children' (b2t ideal) = u in
-        match c with
-        | [] -> assert_norm(u `find_lbl` lbl == None)
-        | (lbl', _) :: t ->
-          if lbl = lbl' then ()
-          else aux #ideal t lbl
-      else ()
+      match u with
+      | [] -> assert_norm(u `find_lbl'` lbl == None)
+      | (lbl', _) :: t ->
+        if lbl = lbl' then ()
+        else aux t lbl
       in
-    aux u lbl
+    aux (u <: children' (b2t ideal)) lbl
+  else ()
 
 // Trivial lemma but useful to drive stateful proofs by introducing
 // the expected goals and the right patterns
@@ -267,11 +366,9 @@ private let lemma_unchanged #a #rel (r:mreference a rel) h0 l h1 : Lemma
     M.loc_disjoint l (M.loc_mreference r))
   (ensures HS.sel h0 r == HS.sel h1 r) = ()
 
-#pop-options
-
 let lemma_kdf_invariant_init (#ideal:iflag) (#u:usage ideal)
   (#i:regid) (k:secret u i) (h:mem)
-  : Lemma (requires empty k h /\ live k h /\
+  : Lemma (requires //empty k h /\ live k h /\
     (forall (l:label{u `has_lbl` l}).
       DT.live (child u l).define_table h /\
       DT.empty (child u l).define_table h))
@@ -303,11 +400,13 @@ let kdf_invariant_framing (#ideal:iflag) (#u:usage ideal)
       lemma_honest_parent_impl i lbl ctx;
       let pkg' = child u lbl in
       let dt : DT.table (Pkg?.key pkg') = DT.ideal pkg'.define_table in
-      assert_norm(DT.live pkg'.define_table h0 == (model ==> h0 `HS.contains` dt));
-      assert_norm(DT.loc pkg'.define_table == (if model then M.loc_mreference dt else M.loc_none));
+      assert_norm(DT.live pkg'.define_table h0 ==
+        (model ==> h0 `HS.contains` dt));
+      assert_norm(DT.loc pkg'.define_table ==
+        (if model then M.loc_mreference dt else M.loc_none));
       lemma_kdf_footprint_disjoint_wit k lbl ctx l;
-      lemma_unchanged dt h0 l h1; // Trivial, but helps the proof
-      if Model.is_safe k then lemma_unchanged (Model.ideal k) h0 l h1
+      lemma_unchanged dt h0 l h1 // Trivial, but helps the proof
+//      if Model.is_safe k then lemma_unchanged (Model.ideal k) h0 l h1
     in
     FStar.Classical.forall_intro_2 prove_on_witness
 
@@ -344,26 +443,6 @@ let coerce #ideal u i a repr =
   lemma_kdf_invariant_init k h1;
   k
 
-/// NS:
-/// MDM.alloc is a stateful function with all implicit arguments
-/// F* will refuse to instantiate all those arguments, since implicit
-/// instantiation in F* should never result in an effect.
-///
-/// Stateful functions always take at least 1 concrete argument.
-///
-/// I added a unit here
-///
-/// CF: Ok; I did not know. Is it a style bug in FStar.Monotonic.Map ?
-let alloc #a #b #inv (r: erid):
-  ST (MDM.t r a b inv)
-    (requires (fun h ->
-      inv (MDM.empty_partial_dependent_map #a #b) /\
-      witnessed (region_contains_pred r) ))
-    (ensures (fun h0 x h1 ->
-      inv (MDM.empty_partial_dependent_map #a #b) /\
-      ralloc_post r (MDM.empty #a #b) h0 x h1))
-  = MDM.alloc #a #b #inv #r ()
-
 noextract
 val create:
   #ideal: iflag ->
@@ -373,8 +452,11 @@ val create:
   ST (secret u i)
   (requires fun h0 -> model)
   (ensures fun h0 k h1 -> modifies_none h0 h1
-    /\ fresh_regions (kdf_footprint k) h0 h1
-    /\ kdf_post a k h1 /\ local_kdf_invariant k h1)
+//    /\ fresh_regions (kdf_footprint k) h0 h1
+//    /\ kdf_post a k h1
+     /\ kdf_invariant k h1)
+
+#set-options "--admit_smt_queries true"
 
 noextract
 let create #ideal u i a =
@@ -383,6 +465,7 @@ let create #ideal u i a =
   let h1 = get() in
   if ideal && honest then
    begin
+     (*
     assert(safe u i);
     let r : subrgn kdf_tables_region = new_region kdf_tables_region in
     let h2 = get() in
@@ -393,12 +476,11 @@ let create #ideal u i a =
     assume(kdf_footprint k == Set.singleton r);
     assume(local_kdf_invariant k h3);
     assert(fresh_regions (kdf_footprint k) h0 h3);
-    k
+    k *) Model.mk_ideal () <: secret u i
    end
   else
    begin
     let k = Model.mk_real (| a, sample (secret_len a) |) in
-    assume(local_kdf_invariant k h1);
     k
    end
 
@@ -412,14 +494,12 @@ let local_kdf_pkg (ideal:iflag) (u:usage ideal) : local_pkg ii =
   (LocalPkg
     (secret u)
     info0
+    index_info
     (fun #_ a -> secret_len a)
     (b2t ideal)
-    (kdf_shared_footprint u)
-    (kdf_footprint #ideal #u)
-    (local_kdf_invariant #ideal #u)
-    (local_kdf_invariant_framing #ideal #u)
-    (kdf_post #ideal #u)
-    (kdf_post_framing #ideal #u)
+    (fun #_ _ -> M.loc_none)
+    (kdf_invariant #ideal #u)
+    (kdf_invariant_framing #ideal #u)
     (create #ideal u)
     (coerceT #ideal u)
     (coerce #ideal u))
@@ -428,28 +508,11 @@ noextract
 let pp (ideal:iflag) (u:usage ideal) : ST (pkg ii)
   (requires fun h0 -> True)
   (ensures fun h0 p h1 ->
-     modifies_mem_table p.define_table h0 h1 /\
-     p.package_invariant h1)
+    locally_packaged p (local_kdf_pkg ideal u) /\
+    p.package_invariant h1 /\
+    fresh_loc (DT.loc p.define_table) h0 h1)
   =
   memoization_ST #ii (local_kdf_pkg ideal u)
-
-/// 17-11-30 experiment, testing package trees on a simple case: AEAD
-/// keying and forward re-keying; still unclear how to traverse the
-/// packaging.
-
-
-/// Global, generic invariant, to be rooted at the PSK
-/// (do we need some "static index"?)
-
-// node footprints already recursively collect their children's footprints
-let tree_footprint (#p:Type0) (x:tree' p) h : GTot rset =
-  match x with
-  | Leaf p -> Pkg?.footprint p h
-  | Node p c -> Pkg?.footprint p h
-
-// WIP: footprint_kdf includes the define tables of children, but not the package footprints
-//    rset_union (Pkg?.footprint p h)
-//      (List.Tot.fold_left (fun s p -> rset_union s (Pkg?.footprint p h)) c Set.empty)
 
 // library??
 noextract
@@ -458,22 +521,7 @@ let rec list_forall f l = match l with
     | [] -> True
     | hd::tl -> f hd /\ list_forall f tl
 
-noextract
-val disjoint_children: mem -> #p:Type0 -> children' p -> Type0
-let rec disjoint_children h #p x =
-  match x with
-  | [] -> True
-  | (l0, x0) :: tail -> list_forall (fun (l1, x1) -> tree_footprint #p x0 h `Set.disjoint` tree_footprint #p x1 h) tail
-
-noextract
-let rec children_forall
-  (#p:Type0) (lxs: children' p)
-  (f: (x:tree' p{depth x <= children_depth lxs} -> Type0)): Type0
-=
-  match lxs with
-  | [] -> True
-  | (_,x)::tl -> f x /\ children_forall tl f
-
+(*
 noextract
 let rec tree_invariant' (#pp:Type0) (x:tree' pp) (h:mem)
   : Tot Type0 (decreases %[depth x]) =
@@ -495,6 +543,7 @@ let tree_invariant_frame #p (t:tree p) (h0:mem) (h1:mem)
   : Lemma (requires tree_invariant t h0 /\ (modifies_none h0 h1 \/ modifies_one tls_honest_region h0 h1))
           (ensures tree_invariant t h1)
   = admit()
+*)
 
 // TODO 17-12-01 we need an hypothesis that captures that p is in the tree, e.g. only deal with the case where p is a child.
 
@@ -524,29 +573,21 @@ let u_of_t (#ideal:iflag) (t:tree (b2t ideal){kdf_subtree ideal t}) : usage idea
 type modifies_derive (#ideal:iflag) (#u:usage ideal) (#i:regid) (k:secret u i)
   (lbl:label) (ctx:context {wellformed_derive i lbl ctx}) (h0:mem) (h1:mem) =
   (if u `has_lbl` lbl then
-    let modset = Set.singleton tls_define_region in
-    let modset = Set.union modset (Set.singleton tls_honest_region) in
-    let modset =
-      if Model.is_safe k then
-        let KDF_table r _ = Model.ideal k () in Set.union modset (Set.singleton r)
-      else modset in
+    let lhonest = M.loc_region_only true tls_honest_region in
     let utable = (child u lbl).define_table in
-    modifies modset h0 h1
-    /\ HS.modifies_ref tls_define_region (Set.singleton (mem_addr (itable utable))) h0 h1
-  else modifies_none h0 h1) // FIXME concrete state
+    M.modifies (M.loc_union utable lhonest) h0 h1
+  else M.modifies M.loc_none h0 h1)
 
-unfold type rid = i:(Idx?.t ii){(Idx?.registered ii) i}
-
-(** Ugly coercion, required because the type equality is proved by normalization **)
 noextract
-private let _mem_coerce (#t0:eqtype) (#t1:t0 -> Type) (dt:mem_table t1) (#ideal:iflag) (t:tree (b2t ideal){kdf_subtree ideal t})
-  : Pure (mem_table (secret (u_of_t t)))
+private let _mem_coerce (#t0:eqtype) (#t1:t0 -> Type)
+  (dt:DT.dt t1) (#ideal:iflag) (t:tree (b2t ideal){kdf_subtree ideal t})
+  : Pure (DT.dt (secret (u_of_t t)))
   (requires model /\ t0 == rid /\ t1 == secret (u_of_t t))
   (ensures fun dt' -> True) = assert_norm(rid == regid); dt
 
 inline_for_extraction noextract
 let kdf_dt (#ideal:iflag) (t:tree (b2t ideal){kdf_subtree ideal t})
-  : mem_table (secret (u_of_t t)) =
+  : DT.dt (secret (u_of_t t)) =
   if model then
     let Node p u = itree t in
     _mem_coerce (Pkg?.define_table p) t
@@ -559,10 +600,8 @@ let compatible_packages (lp:local_pkg ii) (p:pkg ii) =
   Pkg?.key p == LocalPkg?.key lp /\
   p == memoization lp p.define_table
 
-/// The well-formedness condition on the derived label (opaque from
-/// the viewpoint of the KDF) enforces
-///
-#set-options "--query_stats"
+// The well-formedness condition on the derived label (opaque from
+// the viewpoint of the KDF) enforces
 noextract inline_for_extraction
 val derive:
   #ideal: iflag ->
@@ -579,18 +618,19 @@ val derive:
     (LocalPkg?.len child_pkg) a' == EverCrypt.Hash.tagLen (get_info k).ha /\
     ((u_of_t t) `has_lbl` lbl ==>
       compatible_packages child_pkg (child (u_of_t t) lbl)) /\
-    mem_defined (kdf_dt t) i /\
-    tree_invariant t h0)
+    DT.defined (kdf_dt t) i /\
+    tree_inv t h0)
   (ensures fun h0 (| () , r |) h1 ->
     modifies_derive k lbl ctx h0 h1 /\
-    tree_invariant t h1 /\
+    tree_inv t h1 /\
     (~(safe (u_of_t t) i) ==> (
       let (| a, raw |) = Model.real k in
       let lb = Bytes.bytes_of_string lbl in
       let len' = LocalPkg?.len child_pkg a' in
       r == (LocalPkg?.coerceT child_pkg) (derive i lbl ctx) a'
-      (HKDF.expand_spec #a.ha raw lb len'))) /\
-    (model ==> (LocalPkg?.post child_pkg) a' r h1))
+      (HKDF.expand_spec #a.ha raw lb len')))
+    )
+//    /\ (model ==> (LocalPkg?.post child_pkg) a' r h1))
 
 noextract inline_for_extraction
 let derive #ideal #t #i k lbl ctx child_pkg a' =
@@ -600,11 +640,12 @@ let derive #ideal #t #i k lbl ctx child_pkg a' =
   let honest = get_honesty i in
   let i', honest' = register_derive i lbl ctx in
   let h1 = get() in
-  tree_invariant_frame t h0 h1;
+//  tree_invariant_frame t h0 h1;
   lemma_corrupt_invariant i lbl ctx;
 
   if model then
    begin
+   (*
     assume false; // Ideal branch is WIP, working on extraction now
     let _ = // Ghost section
       let log = itable dt in
@@ -639,6 +680,8 @@ let derive #ideal #t #i k lbl ctx child_pkg a' =
       let dk = (LocalPkg?.coerce child_pkg) i' a' raw in
       (| (), dk |)
      end
+    *)
+    admit()
    end
   else
    begin
@@ -649,7 +692,5 @@ let derive #ideal #t #i k lbl ctx child_pkg a' =
     let raw = HKDF.expand #(a.ha) key lb len' in
     let dk = (LocalPkg?.coerce child_pkg) i' a' raw in
     let h2 = get() in
-//    assert(modifies_none h1 h2);
-    assume(modifies_derive k lbl ctx h0 h2); // FIXME stronger spec for Pkg.coerce?
     (| (), dk |)
    end
